

LU factorization

LU factorisation, consists in looking for two matrices L lower triangular, and U upper triangular, both non-singular, such that

$$LU = A \quad (1)$$

If we find these matrices, the original system $A\underline{x} = \underline{b}$ splits into two triangular systems easy to solve:

$$A\underline{x} = \underline{b} \rightarrow L(U\underline{x}) = \underline{b} \rightarrow \begin{cases} L\underline{y} = \underline{b} & \text{solved forward} \\ U\underline{x} = \underline{y} & \text{solved backward} \end{cases}$$

Mathematically equivalent to GEM: matrix U is the same, $\tilde{b} = L^{-1}b$.

LU: unicity of the factors

The factorization $LU = A$ is unique?

$$\underbrace{\begin{bmatrix} l_{11} & 0 & \cdots & 0 \\ l_{21} & l_{22} & \cdots & 0 \\ \vdots & \vdots & & \vdots \\ l_{n1} & l_{n2} & \cdots & l_{nn} \end{bmatrix}}_L \underbrace{\begin{bmatrix} u_{11} & u_{12} & \cdots & u_{1n} \\ 0 & u_{22} & \cdots & u_{2n} \\ \vdots & \vdots & & \vdots \\ 0 & & \cdots & u_{nn} \end{bmatrix}}_U = \underbrace{\begin{bmatrix} a_{11} & a_{12} & \cdots & a_{1n} \\ a_{21} & a_{22} & \cdots & a_{2n} \\ \vdots & \vdots & & \vdots \\ a_{n1} & a_{n2} & \cdots & a_{nn} \end{bmatrix}}_A$$

The unknowns are the coefficients l_{ij} of L , which are

$1 + 2 + \cdots + n = \frac{n(n+1)}{2}$, and the coefficients u_{ij} of U , also $\frac{n(n+1)}{2}$, for a total of $n^2 + n$ unknowns.

We only have n^2 equations (as many as the number of coefficients of A), so we need to fix n unknowns. Usually, the diagonal coefficients of L are set equal to 1: $l_{ii} = 1$. If you do so...

How to compute L and U

Let us introduce Atomic Lower Triangular matrix $L^{(k)}$ defined as

$$L^{(k)} = \begin{bmatrix} 1 & & & & & 0 \\ & \ddots & & & & \\ & & 1 & & & \\ & & -l_{k+1,k} & \ddots & & \\ & & \vdots & & \ddots & \\ 0 & & \underbrace{-l_{n,k}}_{\text{k-th column}} & & & 1 \end{bmatrix}$$

The basic version of GEM can be rewritten in terms of matrix multiplications as:

$$A^{(1)} = A, \quad A^{(2)} = L^{(1)}A, \quad \dots, \quad A^{(n)} = L^{(n-1)}L^{(n-2)} \dots L^{(1)}A = \textcolor{red}{U},$$

where $\textcolor{red}{U}$ is upper triangular.

We observe that

$$L^{(k)-1} = \begin{bmatrix} 1 & & & & 0 \\ & \ddots & & & \\ & & 1 & & \\ & & l_{k+1,k} & \ddots & \\ & & \vdots & & \\ 0 & & \underbrace{l_{n,k}}_{\text{k-th column}} & & 1 \end{bmatrix}, \text{ is still lower triangular}$$

Let us define L as:

$$L := \left(L^{(n-1)} \dots L^{(1)} \right)^{-1} = L^{(1)-1} \dots L^{(n)-1}, \text{ that is still lower triangular}$$

and contains the coefficients $l_{i,k}$ computed in GEM:

$$L = \begin{bmatrix} 1 & 0 & \cdots & 0 \\ l_{2,1} & 1 & \cdots & 0 \\ \vdots & \vdots & & \vdots \\ l_{n,1} & l_{n,2} & \cdots & 1 \end{bmatrix}$$

Recalling that $L^{(n-1)} L^{(n-2)} \dots L^{(1)} A = U$, we obtain $A = LU$.

GEM vs LU (pseudocodes)

GEM

Input: $A \in \mathbb{R}^{n \times n}$ and $b \in \mathbb{R}^n$

for $k = 1, \dots, n-1$

for $i = k+1, \dots, n$

$$l_{i,k} = a_{i,k} / a_{k,k}$$

$$a_{i,k:n} = a_{i,k:n} - l_{i,k} a_{k,k:n}$$

$$b_i = b_i - l_{i,k} b_k$$

end

end

set $U = A$, then solve $Ux = b$ with back substitution

- we can store the $l_{i,k}$ in a matrix:

$$L = \begin{bmatrix} ? & ? & \cdots & ? \\ l_{2,1} & ? & \cdots & ? \\ \vdots & \vdots & & \vdots \\ l_{n,1} & l_{n,2} & \cdots & ? \end{bmatrix}$$

that can be completed as a lower triangular matrix

$$L = \begin{bmatrix} 1 & 0 & \cdots & 0 \\ l_{2,1} & 1 & \cdots & 0 \\ \vdots & \vdots & & \vdots \\ l_{n,1} & l_{n,2} & \cdots & 1 \end{bmatrix}$$

- the loops on the left replace \underline{b} by $L^{-1}\underline{b}$ (see the “equivalent forward substitution” algorithms): $\underline{b} \leftarrow L^{-1}\underline{b}$
- similarly $A \leftarrow L^{-1}A$, which is called U and is an upper triangular matrix:

$$L^{-1}A = U \Rightarrow A = LU$$

GEM vs LU (pseudocodes)

GEM

Input: $A \in \mathbb{R}^{n \times n}$ and $b \in \mathbb{R}^n$

for $k = 1, \dots, n - 1$

for $i = k + 1, \dots, n$

$$l_{i,k} = a_{i,k} / a_{k,k}$$

$$a_{i,k:n} = a_{i,k:n} - l_{i,k} a_{k,k:n}$$

$$b_i = b_i - l_{i,k} b_k$$

end

end

set $U = A$, then solve $Ux = b$ with backward substitution

LU

Input: $A \in \mathbb{R}^{n \times n}$

$$L = I_n \in \mathbb{R}^{n \times n}$$

for $k = 1, \dots, n - 1$

for $i = k + 1, \dots, n$

$$l_{i,k} = a_{i,k} / a_{k,k}$$

$$a_{i,k:n} = a_{i,k:n} - l_{i,k} a_{k,k:n}$$

end

end

Set $U = A$ and output: U and L

Homework

Write the LU algorithm in MATLAB

Permutation matrices

$P \in \mathbb{R}^{n \times n}$ is a permutation matrix if it has only one entry 1 on each row and each column, while the remaining entries are all 0. P produces permutation of rows when multiplying on the left and of columns when multiplying on the right. For example:

$$P = \begin{bmatrix} 0 & 0 & 1 & 0 \\ 1 & 0 & 0 & 0 \\ 0 & 1 & 0 & 0 \\ 0 & 0 & 0 & 1 \end{bmatrix}, \quad A = \begin{bmatrix} \text{---}r_1\text{---} \\ \text{---}r_2\text{---} \\ \text{---}r_3\text{---} \\ \text{---}r_4\text{---} \end{bmatrix} = \begin{bmatrix} | & | & | & | \\ c_1 & c_2 & c_3 & c_4 \\ | & | & | & | \end{bmatrix}$$

$$PA = \begin{bmatrix} 0 & 0 & 1 & 0 \\ 1 & 0 & 0 & 0 \\ 0 & 1 & 0 & 0 \\ 0 & 0 & 0 & 1 \end{bmatrix} \begin{bmatrix} \text{---}r_1\text{---} \\ \text{---}r_2\text{---} \\ \text{---}r_3\text{---} \\ \text{---}r_4\text{---} \end{bmatrix} = \begin{bmatrix} \text{---}r_3\text{---} \\ \text{---}r_1\text{---} \\ \text{---}r_2\text{---} \\ \text{---}r_4\text{---} \end{bmatrix}$$

$$AP = \begin{bmatrix} | & | & | & | \\ c_1 & c_2 & c_3 & c_4 \\ | & | & | & | \end{bmatrix} \begin{bmatrix} 0 & 0 & 1 & 0 \\ 1 & 0 & 0 & 0 \\ 0 & 1 & 0 & 0 \\ 0 & 0 & 0 & 1 \end{bmatrix} = \begin{bmatrix} | & | & | & | \\ c_2 & c_3 & c_1 & c_4 \\ | & | & | & | \end{bmatrix}$$

Remark 1

The product of permutation matrices is still a permutation matrix

GEM: possible troubles and remedy

The condition $\det(A) \neq 0$ is not sufficient to guarantee that the elimination procedure will be successful. For example $A = \begin{bmatrix} 0 & 1 \\ 1 & 0 \end{bmatrix}$

To avoid this the remedy is the “**pivoting**” algorithm:

- **first step**: before eliminating the first column, look for the coefficient of the column biggest in absolute value, the so-called “pivot”; if r is the row where the pivot is found, exchange the first and the r^{th} row.
- **second step**: before eliminating the second column, look for the coefficient of the column biggest in absolute value, starting from the second row; if r is the row where the pivot is found, exchange the second and the r^{th} row.
- \vdots
- **step j** : before eliminating the column j , look for the pivot in this column, from the diagonal coefficient down to the last row. If the pivot is found in the row r , exchange the rows j and r .

This is the pivoting procedure on the rows, which amounts to multiply at the left the matrix A by a permutation matrix P . (An analogous procedure can be applied on the columns, or globally).

Lemma 1

Let $A \in \mathbb{R}^{n \times n}$ be a non singular matrix. Then, at each step of GEM, the “pivot” is not null.

Remark 2

If A is non singular, Lemma 1 ensures that GEM with pivoting can be successfully completed.

The pivoting procedure corresponds then to solve, instead of the original system $\underline{A}\underline{x} = \underline{b}$, the system

$$P\underline{A}\underline{x} = P\underline{b} \quad (2)$$

GEM pseudocode with pivoting

Input as before: $A \in \mathbb{R}^{n \times n}$ and $b \in \mathbb{R}^n$

for $k = 1, \dots, n - 1$

 select $j \geq k$ that maximise $|a_{jk}|$

$a_{j,k:n} \longleftrightarrow a_{k,k:n}$

$b_j \longleftrightarrow b_k$

for $i = k + 1, \dots, n$

$l_{i,k} = a_{i,k} / a_{k,k}$

$a_{i,k:n} = a_{i,k:n} - l_{i,k} a_{k,k:n}$

$b_i = b_i - l_{i,k} b_k$

end

end

define $U = A$, $\tilde{b} = b$, then solve $Ux = \tilde{b}$ with backward substitution

remark: we do not need to define U and \tilde{b} , it is just to be consistent with the notation of the previous slides

LU-continued

GEM and LU have the same computational cost: $\frac{2}{3}n^3$

In GEM, the coefficients l_{ik} are discarded after application to the right-hand side b , while in the LU factorisation they are stored in the matrix L .

If we have to solve a single linear system, GEM is preferable (less memory storage).

If we have to solve many systems with the same matrix and different right-hand sides LU is preferable (the heavy cost is paid only once).

Pivoting is applied also to the LU factorization to ensure that the factorisation is succesful

$$PA = LU \implies PA\underline{x} = P\underline{b} \rightarrow L(U\underline{x}) = P\underline{b} \rightarrow \begin{cases} L\underline{y} = P\underline{b} \\ U\underline{x} = \underline{y} \end{cases}$$

The Matlab function that computes L and U is $lu(.,.)$.

How to compute L , U and P

GEM with pivoting can be rewritten in terms of matrix multiplications as:

$$\begin{aligned} A^{(1)} &= A, & A^{(2)} &= L^{(1)} P^{(1)} A, & \dots, \\ A^{(n)} &= L^{(n-1)} P^{(n-1)} L^{(n-2)} \dots L^{(1)} P^{(1)} A = U, \end{aligned}$$

where U is upper triangular.

Given two generic matrices M, N , it holds $MN \neq NM$, but if $P^{(j)}$ is a permutation matrix that switches i -th and j -th rows, then, for $i \geq j > k$:

$$P^{(j)} L^{(k)} = \tilde{L}^{(k)} P^{(j)},$$

where $\tilde{L}^{(k)}$ is obtained from $L^{(k)}$ by switching $L_{i,k}^{(k)}$ and $L_{j,k}^{(k)}$.

$\tilde{L}^{(k)}$ is still atomic lower triangular, thus $\tilde{L}^{(k)-1}$ is obtained from $\tilde{L}^{(k)}$ by changing signs of the off-diagonal coefficients.

$$\begin{aligned}
U &= L^{(n-1)} P^{(n-1)} L^{(n-2)} P^{(n-2)} L^{(n-3)} \dots L^{(1)} P^{(1)} A \\
&= L^{(n-1)} \tilde{L}^{(n-2)} P^{(n-1)} P^{(n-2)} L^{(n-3)} P^{(n-3)} \dots L^{(1)} P^{(1)} A \\
&= L^{(n-1)} \tilde{L}^{(n-2)} \tilde{\tilde{L}}^{(n-3)} P^{(n-1)} P^{(n-2)} P^{(n-3)} \dots L^{(1)} P^{(1)} A \\
&= \left(L^{(n-1)} \tilde{L}^{(n-2)} \tilde{\tilde{L}}^{(n-3)} \tilde{\tilde{\tilde{L}}}^{(n-4)} \dots \right) P^{(n-1)} P^{(n-2)} P^{(n-3)} \dots P^{(1)} A
\end{aligned}$$

Defining

$$\begin{aligned}
L &= \left(L^{(n-1)} \tilde{L}^{(n-2)} \tilde{\tilde{L}}^{(n-3)} \tilde{\tilde{\tilde{L}}}^{(n-4)} \dots \right)^{-1} \\
P &= P^{(n-1)} P^{(n-2)} P^{(n-3)} \dots P^{(1)}
\end{aligned}$$

we get

$$LU = PA.$$

LU with pivoting (pseudocode)

Input as before: $A \in \mathbb{R}^{n \times n}$

$L = I_n \in \mathbb{R}^{n \times n}$

$P = I_n \in \mathbb{R}^{n \times n}$

for $k = 1, \dots, n - 1$

 select $j \geq k$ that maximise $|a_{jk}|$

$a_{j,k:n} \longleftrightarrow a_{k,k:n}$

$p_{j,:} \longleftrightarrow p_{k,:}$

if $k \geq 2$

$l_{j,1:k-1} \longleftrightarrow l_{k,1:k-1}$

end

for $i = k + 1, \dots, n$

$l_{i,k} = a_{i,k} / a_{k,k}$

$a_{i,k:n} = a_{i,k:n} - l_{i,k} a_{k,k:n}$

end

end

define $U = A$ and output: U , L and P

LU versus GEM

If one needs to compute the inverse of a matrix, LU is the cheapest way. Indeed, recalling the definition, the inverse of a matrix A is the matrix A^{-1} solution of

$$AA^{-1} = I$$

$$\begin{bmatrix} a_{11} & a_{12} & \cdots & a_{1n} \\ a_{21} & a_{22} & \cdots & a_{2n} \\ \vdots & \vdots & & \vdots \\ a_{n1} & a_{n2} & \cdots & a_{nn} \end{bmatrix} \begin{bmatrix} c_{11} & c_{12} & \cdots & c_{1n} \\ c_{21} & c_{22} & \cdots & c_{2n} \\ \vdots & \vdots & & \vdots \\ \underbrace{c_{n1}}_{\underline{c}^{(1)}} & \underbrace{c_{n2}}_{\underline{c}^{(2)}} & \cdots & \underbrace{c_{nn}}_{\underline{c}^{(n)}} \end{bmatrix} = \begin{bmatrix} 1 & 0 & \cdots & 0 \\ 0 & 1 & \cdots & 0 \\ \vdots & \vdots & & \vdots \\ \underbrace{0}_{\underline{e}^1} & \underbrace{0}_{\underline{e}^2} & \cdots & \underbrace{1}_{\underline{e}^n} \end{bmatrix}$$

$$\begin{bmatrix} a_{11} & a_{12} & \cdots & a_{1n} \\ a_{21} & a_{22} & \cdots & a_{2n} \\ \vdots & \vdots & & \vdots \\ a_{n1} & a_{n2} & \cdots & a_{nn} \end{bmatrix} \begin{bmatrix} c_{11} & c_{12} & \cdots & c_{1n} \\ c_{21} & c_{22} & \cdots & c_{2n} \\ \vdots & \vdots & & \vdots \\ \underbrace{c_{n1}}_{\underline{c}^{(1)}} & \underbrace{c_{n2}}_{\underline{c}^{(2)}} & \cdots & \underbrace{c_{nn}}_{\underline{c}^{(n)}} \end{bmatrix} = \begin{bmatrix} 1 & 0 & \cdots & 0 \\ 0 & 1 & \cdots & 0 \\ \vdots & \vdots & & \vdots \\ \underbrace{0}_{\underline{e}^1} & \underbrace{0}_{\underline{e}^2} & \cdots & \underbrace{1}_{\underline{e}^n} \end{bmatrix}$$

Hence, each column $\underline{c}^{(i)}$ of A^{-1} is the solution of

$$A\underline{c}^{(i)} = \underline{e}^{(i)}, \quad i = 1, 2, \dots, n$$

with $\underline{e}^{(i)} = (0, 0, \dots, 1, \dots, 0)$. The factorisation can be done once and for all at the cost of $O(2n^3/3)$ operations; for each column we have to solve 2 triangular systems ($2n^2$ operations) so that the total cost is of the order of $\frac{2}{3}n^3 + n \times 2n^2 = \frac{8}{3}n^3$.

In case of pivoting, we solve $PA\underline{c}^{(i)} = P\underline{e}^{(i)} = P_{:,i}$, $i = 1, 2, \dots, n$.

Computation of the determinant

We can use the LU factorisation to compute the determinant of a matrix. Indeed, if $A = LU$, thanks to the Binet theorem we have

$$\det(A) = \det(L)\det(U) = \prod_{i=1}^n l_{ii} \prod_{i=1}^n u_{ii} = \prod_{i=1}^n u_{ii}$$

Thus the cost to compute the determinant is the same of the LU factorisation.

In the case of pivoting, $PA = LU$ and then

$$\det(A) = \frac{\det(L)\det(U)}{\det(P)} = \frac{\det(U)}{\det(P)}$$

It turns out that $\det(P) = (-1)^\delta$ where $\delta = \#$ of row exchanges in the LU factorisation.

Matlab function: `det(·)`

Cholesky factorization

If A is symmetric ($A = A^T$) and positive definite (positive eigenvalues) a variant of LU is due to Cholesky: there exists a non-singular lower triangular matrix L such that

$$LL^T = A$$

Costs: approximately $\sim \frac{n^3}{3}$ (half the cost of LU, using the symmetry of A).

Matlab function: `chol(.,.)`